src/Enumeration/Iterators.dfy
@@ -1,0 +1,141 @@
+
+include "../Frames.dfy"
+
+module IteratorExperiments {
+
+  import opened Frames
+
+  iterator ForEachWithIndex<T(0)>(s: seq<T>) yields (element: T, index: nat)
+    ensures elements <= s
+    yield ensures elements <= s
+  {
+    for i := 0 to |s|
+      invariant i == |elements|
+      invariant elements <= s
+    {
+      yield s[i], i;
+    }
+  }
+
+  trait Enumerator<T> extends Validatable {
+
+    method MoveNext() returns (more: bool)
+      requires Valid()
+      modifies Repr
+      ensures fresh(Repr - old(Repr))
+      ensures more ==> Valid()
+      ensures more ==> Decreases() < old(Decreases())
+
+    function method Current(): T
+      reads this, Repr
+      requires Valid()
+
+    function Decreases(): nat 
+      reads this, Repr
+      requires Valid()
+  }
+
+  class ForEachWithIndexEnumerator<T(0)> extends Enumerator<(T, nat)> {
+
+    const iter: ForEachWithIndex<T>
+    ghost var remaining: nat
+
+    constructor(s: seq<T>) ensures Valid() ensures fresh(Repr) {
+      iter := new ForEachWithIndex(s);
+      new;
+      remaining := |iter.s|;
+      Repr := {this, iter};
+    }
+
+    predicate Valid() reads this, Repr ensures Valid() ==> this in Repr {
+      && this in Repr
+      && iter in Repr
+      && this !in iter._modifies
+      && this !in iter._reads
+      && this !in iter._new
+      && iter._modifies <= Repr
+      && iter._reads <= Repr
+      && iter._new <= Repr
+      && iter.Valid()
+      && remaining == |iter.s| - |iter.elements|
+    }
+
+    method MoveNext() returns (more: bool) 
+      requires Valid()
+      modifies Repr
+      ensures fresh(Repr - old(Repr))
+      ensures more ==> Valid()
+      ensures more ==> Decreases() < old(Decreases())
+    {
+      more := iter.MoveNext();
+      if (more) {
+        assert old(iter.elements) < iter.elements;
+      }
+      remaining := |iter.s| - |iter.elements|;
+      Repr := {this, iter} + iter._modifies + iter._reads + iter._new;
+    }
+
+    function method Current(): (T, nat) 
+      reads this, Repr
+      requires Valid()
+    {
+      (iter.element, iter.index)
+    }
+
+    function Decreases(): nat reads this, Repr requires Valid() {
+      remaining
+    }
+  }
+
+  method Main() {
+    var s: seq<nat> := [1, 1, 2, 3, 5, 8];
+    var e: Enumerator<(nat, nat)> := new ForEachWithIndexEnumerator(s);
+    assert fresh(e.Repr);
+    label start:
+    var more := true;
+    while (true) 
+      invariant e.Valid()
+      invariant old@start(allocated(e)) && fresh(e.Repr)
+      decreases e.Decreases()
+    {
+      more := e.MoveNext();
+      if (!more) { break; }
+
+      var (element, index) := e.Current();
+      print "Index: ", index, ", Element: ", element;
+    }
+  }
+
+  // iterator Iter<T(0)>(s: set<T>) yields (x: T)
+  //   yield ensures x in s && x !in xs[..|xs|-1];
+  //   ensures s == set z | z in xs;
+  // {
+  //   var r := s;
+  //   while (r != {})
+  //     invariant forall z :: z in xs ==> x !in r;
+  //                                 // r and xs are disjoint
+  //     invariant s == r + set z | z in xs;
+  //   {
+  //     var y :| y in r;
+  //     r, x := r - {y}, y;
+  //     yield;
+  //     assert y == xs[|xs|-1]; // a lemma to help prove loop invariant
+  //   }
+  // }
+
+  // method UseIterToCopy<T(0)>(s: set<T>) returns (t: set<T>)
+  //   ensures s == t;
+  // {
+  //   t := {};
+  //   var m := new Iter(s);
+  //   while (true)
+  //     invariant m.Valid() && fresh(m._new);
+  //     invariant t == set z | z in m.xs;
+  //     decreases s - t;
+  //   {
+  //     var more := m.MoveNext();
+  //     if (!more) { break; }
+  //     t := t + {m.x};
+  //   }
+  // }
+}
